Sompiler simulation, internal diagrams sketched up 1/2

concurrency/compiler/concurrent_compiler_simulation_proof.v
@@ -29,16 +29,15 @@ Module ThreadedSimulation (CC_correct: CompCert_correctness).
   Import DryHybridMachine.
 
   Existing Instance OrdinalPool.OrdinalThreadPool.
+  Existing Instance HybridMachineSig.HybridCoarseMachine.DilMem.
 
   (** *C Semantics*)
   Context (C_program: Clight.program).
   Definition Clight_g : Clight.genv := Clight.globalenv C_program.
   Definition CSem : Semantics := ClightSemantincsForMachines.ClightSem Clight_g.
   Definition Cself_simulation := clight_self_simulation Clight_g.
-  Definition Clight_match := self_simulation.code_inject _ _ Cself_simulation.
-  
-  
-
+  Definition Clight_code_inject := self_simulation.code_inject _ _ Cself_simulation.
+  Definition Clight_match := self_simulation.match_self Clight_code_inject.
   
   (** *Asm Semantics*)
   Import X86Context.
@@ -47,7 +46,8 @@ Module ThreadedSimulation (CC_correct: CompCert_correctness).
   Definition Asm_g := (@the_ge Asm_program).
   Context (Asm_genv_safe: Asm_core.safe_genv (@the_ge Asm_program)).
   Definition Aself_simulation := Asm_self_simulation Asm_g.
-  Definition Asm_match := self_simulation.code_inject _ _ Aself_simulation.
+  Definition Asm_code_inject := self_simulation.code_inject _ _ Aself_simulation.
+  Definition Asm_match := self_simulation.match_self Asm_code_inject.
 
   
   (** *AsHybrid Semantics and Machine*)
@@ -72,7 +72,26 @@ Module ThreadedSimulation (CC_correct: CompCert_correctness).
              CC_correct.CompCert_compiler C_program = Some Asm_program).
   Definition compiler_sim:= CC_correct.simpl_clight_semantic_preservation _ _ compiled.
   Definition compiler_index: Type:= Injindex compiler_sim.
-  Definition compiler_match:= Injmatch_states compiler_sim.
+  Definition compiler_match (i:compiler_index) (j:meminj)
+       (c1:  Smallstep.state (Smallstep.part_sem (Clight.semantics2 C_program)))
+       (m1: mem)
+       (c2: Smallstep.state (Asm.part_semantics Asm_g))
+       (m2: mem): Prop
+    := Injmatch_states compiler_sim i j
+                       (Smallstep.set_mem c1 m1)
+                       (Smallstep.set_mem c2 m2).
+
+  (* Compiler match that holds under interference of other threads. *)
+  Inductive compiler_match_padded:
+    compiler_index -> meminj -> Smallstep.state (Smallstep.part_sem (Clight.semantics2 C_program)) ->
+    mem -> Smallstep.state (Asm.part_semantics Asm_g) -> mem -> Prop
+    :=
+    | BuildCompilerMatch: forall cd j1 j2 j3 j s1 m1 s2 m2 s3 m3 s4 m4,
+        Clight_match j1 s1 m1 s2 m2 ->
+        compiler_match cd j2 s2 m2 s3 m3 ->
+        Asm_match j3 s3 m3 s4 m4 ->
+        compose_meminj (compose_meminj j1 j2) j3 = j ->
+        compiler_match_padded cd j s1 m1 s4 m4.
 
   Context (hb: nat).
   Definition SemTop: Semantics:= (HybridSem (Some hb)).
@@ -85,25 +104,25 @@ Module ThreadedSimulation (CC_correct: CompCert_correctness).
               {sem1 sem2: Semantics}
               (SState: @semC sem1 -> state_sum (@semC CSem) (@semC AsmSem))
               (TState: @semC sem2 -> state_sum (@semC CSem) (@semC AsmSem))
-              set_mem1 set_mem2 (match_state : meminj -> @semC sem1 -> @semC sem2 -> Prop) :
+              (match_state : meminj -> @semC sem1 -> mem -> @semC sem2 -> mem -> Prop) :
     meminj ->
     @ctl (@semC SemTop) -> mem ->
     @ctl (@semC SemBot) -> mem -> Prop  :=
   | CThread_Running: forall j code1 m1 code2 m2,
-      match_state j (set_mem1 code1 m1) (set_mem2 code2 m2) ->
-      match_state2match_thread SState TState set_mem1 set_mem2 match_state j (Krun (SState code1)) m1
+      match_state j code1 m1 code2 m2 ->
+      match_state2match_thread SState TState match_state j (Krun (SState code1)) m1
                             (Krun (TState code2)) m2
   | CThread_Blocked: forall j code1 m1 code2 m2,
-      match_state j (set_mem1 code1 m1) (set_mem2 code2 m2) ->
-      match_state2match_thread SState TState set_mem1 set_mem2 match_state j (Kblocked (SState code1)) m1
+      match_state j code1 m1 code2 m2 ->
+      match_state2match_thread SState TState match_state j (Kblocked (SState code1)) m1
                             (Kblocked (TState code2)) m2
   | CThread_Resume: forall j code1 m1 code2 m2 v v',
-      match_state2match_thread SState TState set_mem1 set_mem2 match_state j (Kresume (SState code1) v) m1
+      match_state2match_thread SState TState match_state j (Kresume (SState code1) v) m1
                             (Kresume (TState code2) v') m2
   | CThread_Init: forall j m1 m2 v1 v1' v2 v2',
       Val.inject j v1 v2 ->
       Val.inject j v1' v2' ->
-      match_state2match_thread SState TState set_mem1 set_mem2 match_state j (Kinit v1 v1') m1
+      match_state2match_thread SState TState match_state j (Kinit v1 v1') m1
                                (Kinit v1 v1') m2.
     
     Definition SST := SState (@semC CSem) (@semC AsmSem).
@@ -112,21 +131,15 @@ Module ThreadedSimulation (CC_correct: CompCert_correctness).
     Definition match_thread_source:
       meminj -> @ctl (@semC SemTop) -> mem -> @ctl (@semC SemBot) -> mem -> Prop:=
       match_state2match_thread SST SST
-                               (@Smallstep.set_mem (Clight.part_semantics2 Clight_g))
-                               (@Smallstep.set_mem (Clight.part_semantics2 Clight_g))
                                Clight_match.
     Definition match_thread_target:
       meminj -> @ctl (@semC SemTop) -> mem -> @ctl (@semC SemBot) -> mem -> Prop:=
       match_state2match_thread TST TST
-                               (@Smallstep.set_mem (Asm.part_semantics Asm_g))
-                               (@Smallstep.set_mem (Asm.part_semantics Asm_g))
                                Asm_match.
     Definition match_thread_compiled cd:
       meminj -> @ctl (@semC SemTop) -> mem -> @ctl (@semC SemBot) -> mem -> Prop:=
       match_state2match_thread SST TST
-                               (@Smallstep.set_mem (Clight.part_semantics2 Clight_g))
-                               (@Smallstep.set_mem (Asm.part_semantics Asm_g))
-                               (compiler_match cd).
+                               (compiler_match_padded cd).
 
     (* NOTE: Old version*)
   (* Inductive match_thread_compiled:
@@ -157,17 +170,12 @@ Module ThreadedSimulation (CC_correct: CompCert_correctness).
       match_thread_compiled cd j (Kinit v1 v1') m1
                             (Kinit v2 v2') m2. *)
     
-  Definition FST {A B} (HH : A /\ B):=
-    fst (ssrfun.pair_of_and HH).
-
-  Definition SND {A B} (HH : A /\ B):=
-    snd (ssrfun.pair_of_and HH).
-    
     Record concur_match (ocd: option compiler_index)
        (j:meminj) (cstate1: ThreadPool (Some hb)) (m1: Mem.mem) (cstate2: ThreadPool(Some (S hb))) (m2: mem):=
   { same_length: num_threads cstate1 = num_threads cstate2
     ; memcompat1: mem_compatible cstate1 m1
     ; memcompat2: mem_compatible cstate2 m2
+    ; taret_invariant: invariant cstate2
     ; mtch_source:
         forall (i:nat),
           (i > hb)%nat ->
@@ -175,9 +183,9 @@ Module ThreadedSimulation (CC_correct: CompCert_correctness).
             (cnti2: containsThread cstate2 i),
           match_thread_source j
                               (getThreadC cnti1)
-                              (permissions.restrPermMap (FST (memcompat1 i cnti1)))
+                              (permissions.restrPermMap (proj1 (memcompat1 i cnti1)))
                               (getThreadC cnti2)
-                              (permissions.restrPermMap (FST (memcompat2 i cnti2)))
+                              (permissions.restrPermMap (proj1 (memcompat2 i cnti2)))
     ; mtch_target:
         forall (i:nat),
           (i < hb)%nat ->
@@ -185,9 +193,9 @@ Module ThreadedSimulation (CC_correct: CompCert_correctness).
             (cnti2: containsThread cstate2 i),
           match_thread_target  j
                               (getThreadC cnti1)
-                              (restrPermMap (FST(memcompat1 i cnti1)))
+                              (restrPermMap (proj1(memcompat1 i cnti1)))
                               (getThreadC cnti2)
-                              (permissions.restrPermMap (FST(memcompat2 i cnti2)))
+                              (permissions.restrPermMap (proj1(memcompat2 i cnti2)))
     ; mtch_compiled:
         forall (i:nat),
           (i = hb)%nat ->
@@ -196,9 +204,9 @@ Module ThreadedSimulation (CC_correct: CompCert_correctness).
             exists cd, ocd = Some cd /\
                   match_thread_compiled cd j
                                         (getThreadC cnti1)
-                                        (restrPermMap (FST(memcompat1 i cnti1)))
+                                        (restrPermMap (proj1 (memcompat1 i cnti1)))
                                         (getThreadC cnti2)
-                                        (restrPermMap (FST(memcompat2 i cnti2))) }.
+                                        (restrPermMap (proj1 (memcompat2 i cnti2))) }.
 
     
     Lemma contains12:
@@ -244,7 +252,7 @@ Module ThreadedSimulation (CC_correct: CompCert_correctness).
     Inductive ord_opt {A} (ord: A -> A -> Prop): option A -> option A -> Prop:=
     | Some_ord:
         forall x y, ord x y -> ord_opt ord (Some x) (Some y).
-      
+    
     Lemma option_wf:
       forall A (ord: A -> A -> Prop),
         well_founded ord ->
@@ -260,8 +268,64 @@ Module ThreadedSimulation (CC_correct: CompCert_correctness).
       inversion H1; subst.
       eapply H0; eauto.
     Qed.
-      
 
+
+    
+    Inductive individual_match ocd i:
+      meminj -> ctl -> mem -> ctl -> mem -> Prop:= 
+    |individual_mtch_source:
+       (i > hb)%nat ->
+       forall j s1 m1 s2 m2,
+         match_thread_source j s1 m1 s2 m2 ->
+         individual_match ocd i j s1 m1 s2 m2
+    |individual_mtch_target:
+       (i < hb)%nat ->
+       forall j s1 m1 s2 m2,
+         match_thread_target j s1 m1 s2 m2 ->
+         individual_match ocd i j s1 m1 s2 m2
+    | individual_mtch_compiled:
+        (i = hb)%nat ->
+        forall cd j s1 m1 s2 m2,
+          ocd = Some cd ->
+          match_thread_compiled cd j s1 m1 s2 m2 ->
+          individual_match ocd i j s1 m1 s2 m2.
+    
+    Lemma Concur_update:
+      forall (st1 : t) (m1 m' : mem) (tid : nat) (Htid : containsThread st1 tid)
+        c1 (cd cd' : option compiler_index) (st2 : t) 
+        (mu : meminj) (m2 : mem)
+        c2
+        (f' : meminj) (m2' : mem) (Htid' : containsThread st2 tid),
+        concur_match cd mu st1 m1 st2 m2 ->
+        individual_match cd' tid f' c1 m' c2 m2' ->
+        self_simulation.is_ext mu (Mem.nextblock m1) f' (Mem.nextblock m2) ->
+        concur_match cd' f'
+                     (updThread Htid c1
+                                (getCurPerm m', snd (getThreadR Htid))) m'
+                     (updThread Htid' c2
+                                (getCurPerm m2', snd (getThreadR Htid'))) m2'.
+    Proof.
+    Admitted.
+
+    
+        Ltac exploit_match:=
+        unfold match_thread_target,match_thread_source,match_thread_compiled in *;
+        match goal with
+        | [ H: getThreadC ?i = _ ?c,
+               H0: context[match_state2match_thread] |- _ ] =>
+          rewrite H in H0; inversion H0; subst; simpl in *
+        end;
+        fold match_thread_target in *;
+        fold match_thread_source in *;
+        fold match_thread_compiled in *.
+
+        (* Build the concur_match *)
+        Ltac destroy_ev_step_sum:=
+          match goal with
+          | [ H: ev_step_sum _ _ _ _ _ _ _ |- _ ] => inversion H; subst
+          end.
+        
+    (* When a thread takes an internal step (i.e. not changing the schedule) *)
     Lemma internal_step_diagram:
       forall (m : option mem) (sge tge : HybridMachineSig.G) (U : list nat)
         (st1 : ThreadPool (Some hb)) (m1 : mem) (st1' : ThreadPool (Some hb)) 
@@ -288,21 +352,51 @@ Module ThreadedSimulation (CC_correct: CompCert_correctness).
       - (* tid < hb *)
         pose proof (mtch_target _ _ _ _ _ _ H0 _ l Htid (contains12 H0 Htid)) as HH.
         simpl in *.
-
-        Ltac exploit_match:=
-        unfold match_thread_target,match_thread_source,match_thread_compiled in *;
-        match goal with
-        | [ H: getThreadC ?i = _ ?c,
-               H0: context[match_state2match_thread] |- _ ] =>
-          rewrite H in H0; inversion H0; subst; simpl in *
-        end;
-        fold match_thread_target in *;
-        fold match_thread_source in *;
-        fold match_thread_compiled in *.
-
         exploit_match.
-        eapply Aself_simulation in H5.
+        destroy_ev_step_sum; simpl in *.
+        simpl.
+        eapply Asm_event.asm_ev_ax1 in H2.
+        replace Hcmpt with (memcompat1 cd mu st1 m1 st2 m2 H0) in H2 by eapply Axioms.proof_irr.
+        instantiate (1:=Asm_genv_safe) in H2.
         
+        eapply Aself_simulation in H5; eauto.
+        destruct H5 as (c2' & f' & t' & m2' & (CoreStep & MATCH & is_ext & inject_incr)).
+
+        (*Try this *)
+        eapply Asm_event.asm_ev_ax2 in CoreStep.
+        destruct CoreStep as (?&?); eauto.
+         
+        (* contains.*)
+        pose proof (@contains12  _ _ _ _ _ _  H0 _ Htid) as Htid'.
+
+        (* Construct the new thread pool *)
+        exists (updThread Htid' (Krun (TState Clight.state Asm.state c2'))
+           (getCurPerm m2', snd (getThreadR Htid'))).
+        (* new memory is given by the self_simulation. *)
+        exists m2', cd, f'. split; [|left].
+        
+        + (*Reestablish the concur_match *)
+          simpl.
+          move H0 at bottom.
+          eapply Concur_update; eauto.
+          econstructor 2; eauto.
+          simpl in MATCH.
+          unfold match_thread_target; simpl.
+          constructor.
+          exact MATCH.
+        + (* Construct the step *)
+          exists 0; simpl.
+          do 2 eexists; split; [|reflexivity].
+          replace m2' with (HybridMachineSig.diluteMem m2') by reflexivity.
+          econstructor; eauto; simpl.
+          econstructor; eauto.
+          * simpl in *.
+            eapply H0.
+          * simpl. econstructor; eauto.
+          * simpl; repeat (f_equal; try eapply Axioms.proof_irr).
+        + eapply Asm_genv_safe.
+      - admit. (*Compiler case*)
+      - 
     Admitted.
 
     Lemma machine_step_diagram:
